src/dafny/smart/Trees2.dfy
@@ -122,51 +122,7 @@ module Trees {
                 leavesIn(lc) + leavesIn(rc) 
     }
 
-    /**
-     *  The node at the end of a path.
-     *
-     *  @param  p   A path (left/right) in a binary tree.
-     *  @param  r   A complete binary tree.
-     *
-     *  @returns    The node of the tree that is the target of path `p`.
-     */
-    function nodeAt(p : seq<bit>, r: ITree) : ITree
-        requires |p| < height(r) 
-        requires isCompleteTree(r)
-        ensures nodeAt(p, r) in nodesIn(r)
-        decreases p
-    {
-        if |p| == 0 then  
-            r
-        else 
-            // r must be a node as height(r) > |p| >= 1
-            match r 
-                case INode(_, lc, rc, _) => 
-                    nodeAt(p[1..], if p[0] == 0 then lc else rc)
-    }
-
-    /**
-     *  The siblings (left or roght) of each node (except root) on the path.
-     */
-    function siblingAt(p : seq<bit>, r :ITree) : ITree
-        requires 1 <= |p| < height(r) 
-        requires isCompleteTree(r)
-        decreases p
-    {
-        if |p| == 1 then
-            match r 
-                case INode(_, lc, rc, _) =>
-                    if p[0] == 0 then rc
-                    else lc
-        else 
-            match r 
-                case INode(_, lc, rc, _) => 
-                    if p[0] == 0 then 
-                        siblingAt(p[1..], lc)
-                    else 
-                        siblingAt(p[1..], rc)
-    }
-
+    
     //  Predicates 
 
    /**
@@ -192,17 +148,17 @@ module Trees {
      *  @param  root    The root node of the tree.
      *  @returns        True if and only if the tree rooted at root is complete
      */
-    predicate isCompleteTree(root : ITree) 
-        decreases root
-    {
-        match root 
-            //  A leaf is a complete tree
-            case ILeaf(_, _) => true
-            //  From a root node, a tree is complete if both children have same height
-            case INode(_, lc, rc, _) => 
-                && height(lc) == height(rc) 
-                && isCompleteTree(lc) && isCompleteTree(rc)
-    }
+    // predicate isCompleteTree(root : ITree) 
+    //     decreases root
+    // {
+    //     match root 
+    //         //  A leaf is a complete tree
+    //         case ILeaf(_, _) => true
+    //         //  From a root node, a tree is complete if both children have same height
+    //         case INode(_, lc, rc, _) => 
+    //             && height(lc) == height(rc) 
+    //             && isCompleteTree(lc) && isCompleteTree(rc)
+    // }
 
     /**
      *  Check that a decorated tree correctly stores the f attribute. 
@@ -247,49 +203,49 @@ module Trees {
      *  The node obtained after a path is the id of rhe node in 
      *  a validIndex tree.
      */
-    lemma {:induction p} nodeIdAtPathIsPath(p : seq<bit>, p': seq<bit>, r: ITree) 
-        requires |p| < height(r) 
-        requires isCompleteTree(r)
-        requires isValidIndex(r, p') 
-        ensures nodeAt(p, r).id == p' + p
-        decreases r
-    {
-        if |p| == 0 {
-            //  Thanks Dafny
-        } else {
-            match r 
-                case INode(_, lc, rc, id) =>
-                    if p[0] == 0 {
-                        //  nodeAt is in lc after p[1..]
-                        nodeIdAtPathIsPath(p[1..], p' + [0], lc);
-                        calc == {
-                            nodeAt(p[1..], lc).id ;
-                            == calc == {
-                                nodeAt(p, r) ;
-                                == 
-                                nodeAt(p[1..], lc);
-                            }
-                            nodeAt(p[1..], lc).id;
-                            ==
-                            p' + [0] + p[1..];
-                        }
-                    } else {   
-                         //  nodeAt is in rc after p[1..]
-                        nodeIdAtPathIsPath(p[1..], p' + [1], rc);
-                        calc == {
-                            nodeAt(p[1..], rc).id ;
-                            == calc == {
-                                nodeAt(p, r) ;
-                                == 
-                                nodeAt(p[1..], rc);
-                            }
-                            nodeAt(p[1..], rc).id;
-                            ==
-                            p' + [1] + p[1..];
-                        }
-                    }
-        }
-    }
+    // lemma {:induction p} nodeIdAtPathIsPath(p : seq<bit>, p': seq<bit>, r: ITree) 
+    //     requires |p| < height(r) 
+    //     requires isCompleteTree(r)
+    //     requires isValidIndex(r, p') 
+    //     ensures nodeAt(p, r).id == p' + p
+    //     decreases r
+    // {
+    //     if |p| == 0 {
+    //         //  Thanks Dafny
+    //     } else {
+    //         match r 
+    //             case INode(_, lc, rc, id) =>
+    //                 if p[0] == 0 {
+    //                     //  nodeAt is in lc after p[1..]
+    //                     nodeIdAtPathIsPath(p[1..], p' + [0], lc);
+    //                     calc == {
+    //                         nodeAt(p[1..], lc).id ;
+    //                         == calc == {
+    //                             nodeAt(p, r) ;
+    //                             == 
+    //                             nodeAt(p[1..], lc);
+    //                         }
+    //                         nodeAt(p[1..], lc).id;
+    //                         ==
+    //                         p' + [0] + p[1..];
+    //                     }
+    //                 } else {   
+    //                      //  nodeAt is in rc after p[1..]
+    //                     nodeIdAtPathIsPath(p[1..], p' + [1], rc);
+    //                     calc == {
+    //                         nodeAt(p[1..], rc).id ;
+    //                         == calc == {
+    //                             nodeAt(p, r) ;
+    //                             == 
+    //                             nodeAt(p[1..], rc);
+    //                         }
+    //                         nodeAt(p[1..], rc).id;
+    //                         ==
+    //                         p' + [1] + p[1..];
+    //                     }
+    //                 }
+    //     }
+    // }
 
     // lemma leaveIdAtPathIsPath(p : seq<bit>, p': seq<bit>, r: ITree) 
     //     requires |p| == height(r) - 1 
@@ -303,98 +259,98 @@ module Trees {
     /**
      *  Index of each node of a indexed tree that is valid is >= `p`.
      */
-    lemma {:induction t} toIndexedIsMonotonic(t : ITree, p : seq<bit>, n : nat)
-        requires isValidIndex(t, p) 
-        requires 0 <= n < |nodesIn(t)|
-        /** Weak ordering for all nodes. */
-        ensures p <= nodesIn(t)[n].id 
-        /** For nodes in lc and rc, strict prefix ordering wrt root.id.. */
-        ensures n >= 1 ==> p < nodesIn(t)[n].id 
-        decreases t 
-    {
-        match t 
-            case ILeaf(_, _) =>
+    // lemma {:induction t} toIndexedIsMonotonic(t : ITree, p : seq<bit>, n : nat)
+    //     requires isValidIndex(t, p) 
+    //     requires 0 <= n < |nodesIn(t)|
+    //     /** Weak ordering for all nodes. */
+    //     ensures p <= nodesIn(t)[n].id 
+    //     /** For nodes in lc and rc, strict prefix ordering wrt root.id.. */
+    //     ensures n >= 1 ==> p < nodesIn(t)[n].id 
+    //     decreases t 
+    // {
+    //     match t 
+    //         case ILeaf(_, _) =>
 
-            case INode(_, lc, rc, _) => 
-                if ( n == 0 ) {
-                    //  Thanks Dafny
-                }  else if ( 1 <= n <= |nodesIn(lc)|) {
-                    toIndexedIsMonotonic(lc, p + [0], n - 1);
-                } else {
-                    toIndexedIsMonotonic(rc, p + [1], n - 1 - |nodesIn(lc)|);
-                }
-    }
+    //         case INode(_, lc, rc, _) => 
+    //             if ( n == 0 ) {
+    //                 //  Thanks Dafny
+    //             }  else if ( 1 <= n <= |nodesIn(lc)|) {
+    //                 toIndexedIsMonotonic(lc, p + [0], n - 1);
+    //             } else {
+    //                 toIndexedIsMonotonic(rc, p + [1], n - 1 - |nodesIn(lc)|);
+    //             }
+    // }
 
     /**
      *  Each node has a unique id in a validIndexed tree.
      */
-    lemma {:induction r} eachNodeHasUniqueId(r: ITree, k1 : nat, k2 : nat, p : seq<bit>) 
-        requires isValidIndex(r, p) 
-        /** Two arbitrary strictly ordered indices within the range of nodesIn  */
-        requires 0 <= k1 < k2 < |nodesIn(r)|
-        /** The ids of two arbitary nodes are not equal. */
-        ensures nodesIn(r)[k1].id !=  nodesIn(r)[k2].id
-        decreases r
-    { 
-        match r 
-            case ILeaf(v, id) => // Vacuously true. Thanks Dafny
+    // lemma {:induction r} eachNodeHasUniqueId(r: ITree, k1 : nat, k2 : nat, p : seq<bit>) 
+    //     requires isValidIndex(r, p) 
+    //     /** Two arbitrary strictly ordered indices within the range of nodesIn  */
+    //     requires 0 <= k1 < k2 < |nodesIn(r)|
+    //     /** The ids of two arbitary nodes are not equal. */
+    //     ensures nodesIn(r)[k1].id !=  nodesIn(r)[k2].id
+    //     decreases r
+    // { 
+    //     match r 
+    //         case ILeaf(v, id) => // Vacuously true. Thanks Dafny
 
-            case INode(v, lc, rc, id) =>
+    //         case INode(v, lc, rc, id) =>
 
-                if ( k1 == 0 ) {
-                    //  k2 is an index of a node in lc or rc, strict ordering applies.
-                    toIndexedIsMonotonic(r, p, k2);
-                } else if 1 <= k1 < k2 <= |nodesIn(lc)| {
-                    //  both indices are nodes in lc. Use induction hypothesis on lc.
-                    eachNodeHasUniqueId(lc, k1 - 1, k2 - 1, p + [0]);
-                } else if 1 + |nodesIn(lc)| <= k1 < k2 < |nodesIn(r)| {
-                    //  both indices are nodes in rc. Use induction hypothesis on rc. 
-                    var i1 := k1 - 1 - |nodesIn(lc)|;
-                    var i2 := k2 - 1 - |nodesIn(lc)|;
-                    eachNodeHasUniqueId(rc, i1, i2, p + [1]);   
-                } else {
-                    //  k1 indexes a node in lc.
-                    assert ( 1 <= k1 <= 1 + |nodesIn(lc)| <= k2 < |nodesIn(r)| );
-                    var i1 := k1 - 1;
-                    //  Use induction hypothesis on lc. ids on nodes in lc >= p + [0]
-                    toIndexedIsMonotonic(lc, p + [0], i1);
+    //             if ( k1 == 0 ) {
+    //                 //  k2 is an index of a node in lc or rc, strict ordering applies.
+    //                 toIndexedIsMonotonic(r, p, k2);
+    //             } else if 1 <= k1 < k2 <= |nodesIn(lc)| {
+    //                 //  both indices are nodes in lc. Use induction hypothesis on lc.
+    //                 eachNodeHasUniqueId(lc, k1 - 1, k2 - 1, p + [0]);
+    //             } else if 1 + |nodesIn(lc)| <= k1 < k2 < |nodesIn(r)| {
+    //                 //  both indices are nodes in rc. Use induction hypothesis on rc. 
+    //                 var i1 := k1 - 1 - |nodesIn(lc)|;
+    //                 var i2 := k2 - 1 - |nodesIn(lc)|;
+    //                 eachNodeHasUniqueId(rc, i1, i2, p + [1]);   
+    //             } else {
+    //                 //  k1 indexes a node in lc.
+    //                 assert ( 1 <= k1 <= 1 + |nodesIn(lc)| <= k2 < |nodesIn(r)| );
+    //                 var i1 := k1 - 1;
+    //                 //  Use induction hypothesis on lc. ids on nodes in lc >= p + [0]
+    //                 toIndexedIsMonotonic(lc, p + [0], i1);
 
-                    //  k2 indexes a node in rc.
-                    var i2 := k2 - 1 - |nodesIn(lc)|;
-                    //  Use induction hypothesis on rc. Ids of nodes in rc >= p + [1]
-                    toIndexedIsMonotonic(rc, p + [1], i2);
+    //                 //  k2 indexes a node in rc.
+    //                 var i2 := k2 - 1 - |nodesIn(lc)|;
+    //                 //  Use induction hypothesis on rc. Ids of nodes in rc >= p + [1]
+    //                 toIndexedIsMonotonic(rc, p + [1], i2);
 
-                    //  Prove post condition by contradiction. 
-                    //  Idea: lc nodes start with p + [0] and rc nodes with p + [1].
-                    //  Turns out that p + [0] + p' != p + [1] + p' for all p'.
-                    calc ==> {
-                        nodesIn(r)[k1].id == nodesIn(r)[k2].id ;
-                        ==>
-                        nodesIn(r)[k1].id[..|p| + 1] == nodesIn(r)[k2].id[..|p| + 1] ;
-                        ==> calc == {
-                                p + [0] ;
-                                ==
-                                (p + [0])[..|p| + 1];
-                                == 
-                                nodesIn(r)[k1].id[..|p| + 1];
-                        }
-                        p + [0] == nodesIn(r)[k2].id[..|p| + 1] ;
-                        ==> calc == {
-                                p + [1] ;
-                                ==
-                                (p + [1])[..|p| + 1];
-                                == 
-                                nodesIn(r)[k2].id[..|p| + 1];
-                        }
-                        p + [0] == p + [1];
-                        ==>
-                        (p + [0])[|p|] == (p + [1])[|p|];
-                        ==>
-                        //  contradiction
-                        0 == 1;
-                    }
-                } 
-    }
+    //                 //  Prove post condition by contradiction. 
+    //                 //  Idea: lc nodes start with p + [0] and rc nodes with p + [1].
+    //                 //  Turns out that p + [0] + p' != p + [1] + p' for all p'.
+    //                 calc ==> {
+    //                     nodesIn(r)[k1].id == nodesIn(r)[k2].id ;
+    //                     ==>
+    //                     nodesIn(r)[k1].id[..|p| + 1] == nodesIn(r)[k2].id[..|p| + 1] ;
+    //                     ==> calc == {
+    //                             p + [0] ;
+    //                             ==
+    //                             (p + [0])[..|p| + 1];
+    //                             == 
+    //                             nodesIn(r)[k1].id[..|p| + 1];
+    //                     }
+    //                     p + [0] == nodesIn(r)[k2].id[..|p| + 1] ;
+    //                     ==> calc == {
+    //                             p + [1] ;
+    //                             ==
+    //                             (p + [1])[..|p| + 1];
+    //                             == 
+    //                             nodesIn(r)[k2].id[..|p| + 1];
+    //                     }
+    //                     p + [0] == p + [1];
+    //                     ==>
+    //                     (p + [0])[|p|] == (p + [1])[|p|];
+    //                     ==>
+    //                     //  contradiction
+    //                     0 == 1;
+    //                 }
+    //             } 
+    // }
     
     /**
      *  Collect nodes on the right hand-side of a full path.
@@ -479,72 +435,72 @@ module Trees {
     // }
 
 
-    //  Helpers lemmas for complete trees.
+    // //  Helpers lemmas for complete trees.
 
-    /**
-     *  Relation between height and number of leaves in a complete tree.
-     */
-    lemma {:induction root} completeTreeNumberLemmas(root : ITree) 
-        ensures isCompleteTree(root) ==> |leavesIn(root)| == power2(height(root) - 1)
-        ensures isCompleteTree(root) ==> |nodesIn(root)| == power2(height(root)) - 1
-    {   //  Thanks Dafny
-    }
+    // /**
+    //  *  Relation between height and number of leaves in a complete tree.
+    //  */
+    // lemma {:induction root} completeTreeNumberLemmas(root : ITree) 
+    //     ensures isCompleteTree(root) ==> |leavesIn(root)| == power2(height(root) - 1)
+    //     ensures isCompleteTree(root) ==> |nodesIn(root)| == power2(height(root)) - 1
+    // {   //  Thanks Dafny
+    // }
 
-    /**
-     *  Two complete tree of same height have same number of leaves.
-     */
-    lemma {:induction r1, r2} completeTreesOfSameHeightHaveSameNumberOfLeaves(r1: ITree, r2: ITree) 
-        requires isCompleteTree(r1)
-        requires isCompleteTree(r2)
-        ensures height(r1) == height(r2) ==> |leavesIn(r1)| == |leavesIn(r2)|
-    {   //  Thanks Dafny
-    }
+    // /**
+    //  *  Two complete tree of same height have same number of leaves.
+    //  */
+    // lemma {:induction r1, r2} completeTreesOfSameHeightHaveSameNumberOfLeaves(r1: ITree, r2: ITree) 
+    //     requires isCompleteTree(r1)
+    //     requires isCompleteTree(r2)
+    //     ensures height(r1) == height(r2) ==> |leavesIn(r1)| == |leavesIn(r2)|
+    // {   //  Thanks Dafny
+    // }
 
-    /**
-     *  Children of a node in a complete tree have same number of leaves.
-     */
-    lemma {:induction r} completeTreesLeftRightHaveSameNumberOfLeaves(r : ITree) 
-        requires isCompleteTree(r)
-        requires height(r) >= 2
-        ensures match r
-            case INode(_, lc, rc, _) => 
-                |leavesIn(lc)| == |leavesIn(rc)| == power2(height(r) - 1) / 2
-    {
-        match r 
-            case INode(_, lc, rc, _) =>
-                completeTreesOfSameHeightHaveSameNumberOfLeaves(lc,rc);
-    }
+    // /**
+    //  *  Children of a node in a complete tree have same number of leaves.
+    //  */
+    // lemma {:induction r} completeTreesLeftRightHaveSameNumberOfLeaves(r : ITree) 
+    //     requires isCompleteTree(r)
+    //     requires height(r) >= 2
+    //     ensures match r
+    //         case INode(_, lc, rc, _) => 
+    //             |leavesIn(lc)| == |leavesIn(rc)| == power2(height(r) - 1) / 2
+    // {
+    //     match r 
+    //         case INode(_, lc, rc, _) =>
+    //             completeTreesOfSameHeightHaveSameNumberOfLeaves(lc,rc);
+    // }
 
-    lemma {:induction r} completeTreesLeftRightChildrenLeaves(r : ITree, h : nat) 
-        requires isCompleteTree(r)
-        requires h == height(r) >= 2
-        ensures |leavesIn(r)| == power2(h - 1)
-        ensures match r
-            case INode(_, lc, rc, _) => 
-                leavesIn(lc) == leavesIn(r)[.. power2(h - 1) / 2]
-                && leavesIn(rc) == leavesIn(r)[power2(height(r) - 1) / 2 ..]
-    {
-        if h == 2 {
-            //  Thanks Dafny
-        } else {
-            match r
-                case INode(_, lc, rc, _) => 
-                    completeTreesLeftRightHaveSameNumberOfLeaves(r);
-        }
-    }
+    // lemma {:induction r} completeTreesLeftRightChildrenLeaves(r : ITree, h : nat) 
+    //     requires isCompleteTree(r)
+    //     requires h == height(r) >= 2
+    //     ensures |leavesIn(r)| == power2(h - 1)
+    //     ensures match r
+    //         case INode(_, lc, rc, _) => 
+    //             leavesIn(lc) == leavesIn(r)[.. power2(h - 1) / 2]
+    //             && leavesIn(rc) == leavesIn(r)[power2(height(r) - 1) / 2 ..]
+    // {
+    //     if h == 2 {
+    //         //  Thanks Dafny
+    //     } else {
+    //         match r
+    //             case INode(_, lc, rc, _) => 
+    //                 completeTreesLeftRightHaveSameNumberOfLeaves(r);
+    //     }
+    // }
 
     /**
      *  If the id of root is [], then each node n.id is the path
      *  from root to n.
      */
-    lemma {:induction r} nodeAtCanonicalPath(p : seq<bit>, r : ITree) 
-         requires |p| < height(r) 
-        requires isCompleteTree(r)
-        requires isValidIndex(r, [])
-        ensures nodeAt(p, r).id == p 
-    {
-        nodeIdAtPathIsPath(p, [], r);
-    } 
+    // lemma {:induction r} nodeAtCanonicalPath(p : seq<bit>, r : ITree) 
+    //      requires |p| < height(r) 
+    //     requires isCompleteTree(r)
+    //     requires isValidIndex(r, [])
+    //     ensures nodeAt(p, r).id == p 
+    // {
+    //     nodeIdAtPathIsPath(p, [], r);
+    // } 
 
     // lemma {:induction r} foo201(r: ITree, p: seq<bit>, lc1: ITree) 
     //     requires height(r) >= 2
@@ -571,32 +527,7 @@ module Trees {
     //                 nodeAtCanonicalPath(p[1..], lc);   
     // }
 
-    lemma nodeLoc(r : ITree, p : seq<bit>) 
-        requires 1 <= |p| == height(r) - 1
-        requires isCompleteTree(r)
-
-        ensures match r 
-            case INode(_, lc, rc, _) =>
-                p[0] == 0 ==> nodeAt(p, r) in leavesIn(lc)
-                &&
-                p[0] == 1 ==> nodeAt(p, r) in leavesIn(rc)
-
-    lemma nodeLoc2(r : ITree, p : seq<bit>, k : nat) 
-        requires 1 <= |p| == height(r) - 1
-        requires isCompleteTree(r)
-        // requires isValidIndex(r, p')
-        requires k < power2(height(r) - 1)
-        requires k < |leavesIn(r)|
-        // requires nodeAt(p, r).id == leavesIn(r)[k].id
-        // requires p' + p == leavesIn(r)[k].id
-        // requires nodeAt(p, r) == leavesIn(r)[k]
-
-        ensures match r 
-            case INode(_, lc, rc, _) =>
-                (p[0] == 0 && k < power2(height(r) - 1)/2)
-                ||
-                (p[0] == 1 && k >= power2(height(r) - 1)/2)
-
+    
    
     // function binToNat(p : seq<bit>) : nat 
     //     requires |p| >= 1
@@ -724,310 +655,62 @@ module Trees {
     //     ensures |p| >= 1 && p[0] == 1 ==> bitListToNat(p) == power2(|p| - 1) + bitListToNat(p[1..])
     // {}
 
-    lemma foo302(p : seq<bit>, r : ITree, k : nat) 
-        requires isCompleteTree(r)
-        requires 1 <= |p| == height(r) - 1 
-        requires k < |leavesIn(r)|
-        requires nodeAt(p, r) == leavesIn(r)[k]
-        ensures bitListToNat(p) == k
-    {
-        if |p| == 1 {
-            if p[0] == 0 {
-                nodeLoc2(r, p, k);
-                assert(k == 0);
-                assert(bitListToNat(p) == 0);
-                assert(nodeAt(p, r) == leavesIn(r)[0]);
-            } else {
-                assert(p[0] == 1);
-                nodeLoc2(r, p, k);
-                assert(k == 1);
-                assert(bitListToNat(p) == 1);
-                assert(nodeAt(p, r) == leavesIn(r)[k]);
-            }
-        } else {
-            //  r is not a leaf
-            match r 
-                case INode(_, lc, rc, _) => 
-                    if p[0] == 0 {
-                        //  left lc
-                        assert(nodeAt(p, r) == nodeAt(p[1..], lc));
-                        //  HI on rc
-                        completeTreesLeftRightHaveSameNumberOfLeaves(r);
-                        nodeLoc2(r, p, k);
-                        assert( k < power2(height(r) - 1)/ 2);
-                        assert(|leavesIn(lc)| == power2(height(r) - 1)/ 2);
-                        // foo302(p[1..], lc, k);
-                    } else {
-                        //  p[0] == 1
-                        assert(nodeAt(p, r) == nodeAt(p[1..], rc));
-                        completeTreesLeftRightHaveSameNumberOfLeaves(r);
-                        nodeLoc2(r, p, k);
-                        assert( k >= power2(height(r) - 1)/ 2);
-                        assert(|leavesIn(rc)| == power2(height(r) - 1)/ 2);
-                        var k' := k - power2(height(r) - 1)/ 2 ;
-                        foo302(p[1..], rc, k');
-                    }
-        }
-    }
+    // lemma foo302(p : seq<bit>, r : ITree, k : nat) 
+    //     requires isCompleteTree(r)
+    //     requires 1 <= |p| == height(r) - 1 
+    //     requires k < |leavesIn(r)|
+    //     requires nodeAt(p, r) == leavesIn(r)[k]
+    //     ensures bitListToNat(p) == k
+    // {
+    //     if |p| == 1 {
+    //         if p[0] == 0 {
+    //             nodeLoc2(r, p, k);
+    //             assert(k == 0);
+    //             assert(bitListToNat(p) == 0);
+    //             assert(nodeAt(p, r) == leavesIn(r)[0]);
+    //         } else {
+    //             assert(p[0] == 1);
+    //             nodeLoc2(r, p, k);
+    //             assert(k == 1);
+    //             assert(bitListToNat(p) == 1);
+    //             assert(nodeAt(p, r) == leavesIn(r)[k]);
+    //         }
+    //     } else {
+    //         //  r is not a leaf
+    //         match r 
+    //             case INode(_, lc, rc, _) => 
+    //                 if p[0] == 0 {
+    //                     //  left lc
+    //                     assert(nodeAt(p, r) == nodeAt(p[1..], lc));
+    //                     //  HI on rc
+    //                     completeTreesLeftRightHaveSameNumberOfLeaves(r);
+    //                     nodeLoc2(r, p, k);
+    //                     assert( k < power2(height(r) - 1)/ 2);
+    //                     assert(|leavesIn(lc)| == power2(height(r) - 1)/ 2);
+    //                     // foo302(p[1..], lc, k);
+    //                 } else {
+    //                     //  p[0] == 1
+    //                     assert(nodeAt(p, r) == nodeAt(p[1..], rc));
+    //                     completeTreesLeftRightHaveSameNumberOfLeaves(r);
+    //                     nodeLoc2(r, p, k);
+    //                     assert( k >= power2(height(r) - 1)/ 2);
+    //                     assert(|leavesIn(rc)| == power2(height(r) - 1)/ 2);
+    //                     var k' := k - power2(height(r) - 1)/ 2 ;
+    //                     foo302(p[1..], rc, k');
+    //                 }
+    //     }
+    // }
 
-     lemma foo203(p : seq<bit>, r : ITree, k : nat) 
-        requires isCompleteTree(r)
-        requires 1 <= |p| == height(r) - 1 
-        requires k < |leavesIn(r)|
-        requires bitListToNat(p) == k
-        ensures nodeAt(p, r) == leavesIn(r)[k]
-        decreases p 
-    {
-        if |p| == 1 {
-            if p[0] == 0 {
-                nodeLoc2(r, p, k);
-                assert(k == 0);
-                assert(bitListToNat(p) == 0);
-                assert(nodeAt(p, r) == leavesIn(r)[0]);
-            } else {
-                assert(p[0] == 1);
-                nodeLoc2(r, p, k);
-                assert(k == 1);
-                assert(bitListToNat(p) == 1);
-                assert(nodeAt(p, r) == leavesIn(r)[k]);
-            }
-        } else {
-            //  r is not a leaf
-            match r 
-                case INode(_, lc, rc, _) => 
-                    if p[0] == 0 {
-                        //  left lc
-                        assert(nodeAt(p, r) == nodeAt(p[1..], lc));
-                        //  HI on rc
-                        completeTreesLeftRightHaveSameNumberOfLeaves(r);
-                        nodeLoc2(r, p, k);
-                        assert( k < power2(height(r) - 1)/ 2);
-                        assert(|leavesIn(lc)| == power2(height(r) - 1)/ 2);
-                        // foo302(p[1..], lc, k);
-                    } else {
-                        //  p[0] == 1
-                        assert(nodeAt(p, r) == nodeAt(p[1..], rc));
-                        completeTreesLeftRightHaveSameNumberOfLeaves(r);
-                        nodeLoc2(r, p, k);
-                        assert( k >= power2(height(r) - 1)/ 2);
-                        assert(|leavesIn(rc)| == power2(height(r) - 1)/ 2);
-                        var k' := k - power2(height(r) - 1)/ 2 ;
-                        foo203(p[1..], rc, k');
-                        // assume( nodeAt(p, r) == leavesIn(r)[k]);
-                    }
-        }
-    }
+    
 
-    lemma foo200(p : seq<bit>, r : ITree, k : nat) 
-        requires isCompleteTree(r)
-        requires 1 <= |p| == height(r) - 1 
-        requires k < |leavesIn(r)|
-        ensures bitListToNat(p) == k <==> nodeAt(p, r) == leavesIn(r)[k]
-    {
-        if (bitListToNat(p) == k) {
-            foo203(p, r, k);
-        } else if ( nodeAt(p, r) == leavesIn(r)[k]) {
-            foo302(p, r, k);
-        }
-        
-    }
-
-    /**
-     *  A path to a leaf of index < |leavesin{r)| -1 has a zero in it.
-     */
-    lemma {:induction p} pathToLeafInInitHasZero(p: seq<bit>, r : ITree, k : nat)
-        requires |p| == height(r) - 1
-        requires isCompleteTree(r)
-        requires k < |leavesIn(r)| - 1
-        requires nodeAt(p, r) == leavesIn(r)[k]
-        ensures exists i :: 0 <= i < |p| && p[i] == 0
-        decreases p 
-    {
-        if |p| == 1 {
-            //  k < |leavesIn(r)| <==> k < 1 <==> k == 0, apply nodeLoc2 ==> p[0] == 0
-            nodeLoc2(r, p, k);
-        } else {
-            if p[0] == 0 {
-                //  p[0] is a witness
-            } else {
-                //  r is a node (not a leaf) and path leads to a node in rc
-                match r
-                    case INode(_, lc, rc, _) =>
-                        completeTreeNumberLemmas(r);
-                        assert(|leavesIn(r)| == power2(height(r) - 1));
-                        assert( k < power2(height(r) - 1));
-                        //  k >= power2(height(r) -1 ) /2 by
-                        nodeLoc2(r, p, k);
-                        //  leavesIn(r)[k] == leavesIn(rc)[k - power2(height(r) - 1)/2]
-                        completeTreesLeftRightChildrenLeaves(r, height(r));
-                        var k' := k - power2(height(r) - 1) / 2;
-                        assert(leavesIn(r)[k] == leavesIn(rc)[k']);
-                        completeTreesLeftRightHaveSameNumberOfLeaves(r);
-                        //  induction on rc
-                        pathToLeafInInitHasZero(p[1..], rc, k');
-            }
-        }
-    }
+   
     //  Synthesised attibutes Helpers
 
     // function decoratePath(r: ITree, l : seq<bit>, )
 
-    //  Some properties of adjacent path
+    
 
-    /** Compute a path (supposedly to next leaf, to prove!) */
-    function nextPath(p : seq<bit>) : seq<bit> 
-        /** Path has at least on element. */
-        requires |p| >= 1
-        /** Not the path 1+ that has no successors. */
-        requires exists i :: 0 <= i < |p| && p[i] == 0
-        ensures |nextPath(p)| == |p|
-
-        decreases p
-    {
-        if p[|p| - 1] == 0 then 
-            p[..|p| - 1] + [1]
-        else 
-           nextPath(p[.. |p| - 1]) + [0]
-    }
-
-    lemma nextPathIsSucc(p : seq<bit>)
-         /** Path has at least on element. */
-        requires |p| >= 1
-        /** Note the path 1+ that has no successors. */
-        requires exists i :: 0 <= i < |p| && p[i] == 0
-        ensures bitListToNat(nextPath(p)) == bitListToNat(p) + 1
-    {
-        if |p| == 1 {
-            //  Thanks Dafny
-        } else {
-            if p[|p| - 1] == 0 {
-                assert(nextPath(p) == p[..|p| - 1] + [1]);
-                assert( p == p[..|p| - 1] + [0]);
-                foo101(p[..|p| - 1], 0);
-                assert(bitListToNat(p) == 2 * bitListToNat(p[..|p| - 1]));
-                foo101(p[..|p| - 1], 1);
-                assert(bitListToNat(nextPath(p)) == 2 * bitListToNat(p[..|p| - 1]) + 1);
-            } else {
-                //  last of p is 1
-                assert( p == p[..|p| - 1] + [1]);
-
-                //  def of next path
-                assert(nextPath(p) == nextPath(p[..|p| - 1]) + [0]);
-                assert(p[|p| - 1] == 1);
-
-                assert(exists i :: 0 <= i < |p| && i != |p| - 1 && p[i] == 0);
-              
-                assert(exists i :: 0 <= i < |p| - 1 && p[i] == 0);
-                assert(exists i :: 0 <= i < |p[..|p| - 1]| && p[..|p| - 1][i] == 0);
-                // //  Induction on p[..|p| - 1]
-                assert(bitListToNat(nextPath(p[..|p| - 1])) == bitListToNat(p[..|p| - 1]) + 1);
-                // //  binListToNat2 suffix
-                foo101(p[..|p| - 1], 1);
-                assert( bitListToNat(p) == 2 * bitListToNat(p[..|p| - 1]) + 1);
-
-                calc {
-                    bitListToNat(nextPath(p));
-                    == 
-                    bitListToNat(nextPath(p[..|p| - 1]) + [0]);
-                    == { foo101(nextPath(p[..|p| - 1]), 0);}
-                    2 * bitListToNat(nextPath(p[..|p| - 1]));
-                    == { nextPathIsSucc(p[..|p| - 1]) ; } 
-                    2 * (bitListToNat(p[..|p| - 1]) + 1) ;
-                    ==
-                    2 * bitListToNat(p[..|p| - 1]) + 2 ;
-                    ==
-                    (2 * bitListToNat(p[..|p| - 1]) + 1) + 1 ;
-                    ==
-                    bitListToNat(p) + 1;
-                }
-            }
-        }
-    } 
-
-    /**
-     *  A path to a leaf which is not the rightmost one must have 
-     *  a zero.
-     */
-    lemma {:induction p} foo450(p: seq<bit>, r : ITree, k : nat) 
-        requires isCompleteTree(r)
-        requires 1 <= |p| == height(r) - 1
-        requires 0 <= k < |leavesIn(r)| - 1
-        requires nodeAt(p, r) == leavesIn(r)[k]
-        ensures  exists i ::  0 <= i < |p| && p[i] == 0 
-        decreases p 
-    {
-        if |p| == 1 {
-            //  Thanks Dafny
-            assert(k == 0);
-            nodeLoc2(r, p, k);
-            assert(p[0] == 0);
-        } else {
-            if p[0] == 0 {
-                //  
-            } else {
-                // p[0] == 1, apply to rc
-                match r
-                    case INode(_, _, rc, _) =>
-                        assert(isCompleteTree(rc));
-                        assert(1 <= |p[1..]|);
-                        assert(nodeAt(p, r) == nodeAt(p[1..], rc));
-                        // assert(|leavesIn(rc)| == )
-                        completeTreesLeftRightHaveSameNumberOfLeaves(r);
-                        assert(p[0] == 1);
-                        nodeLoc2(r, p, k);
-                        assert( 0 <= k - power2(height(r) - 1) / 2);
-                        assert( k - power2(height(r) - 1)/ 2 < |leavesIn(rc)| - 1);
-                        foo450(p[1..], rc, k - power2(height(r) - 1)/2);
-                        assert(exists i ::  0 <= i < |p[1..]| && p[1..][i] == 0); 
-                        // var i :|  0 <= i < |p[1..]| && p[1..][i] == 0 ;
-            }
-        }
-    } 
-
-    // lemma foo201(p: seq<bit>, r : ITree, k : nat )
-    //     requires isCompleteTree(r)
-    //     requires 2 <= |p| == height(r) - 1
-    //     requires 0 <= k < (|leavesIn(r)| - 1)/2 - 1
-    //     requires nodeAt(p, r) == leavesIn(r)[k]
-    //     // ensures  exists i ::  0 <= i < |p| && p[i] == 0 
-    //     decreases p 
-    //     ensures exists i ::  0 <= i < |p| && p[i] == 0 
-    //     ensures match r 
-    //         case INode(_, lc, rc, _) =>
-    //             (exists i ::  0 <= i < |p| && p[i] == 0 )
-    //             && nodeAt(nextPath(p), r) == nodeAt(nextPath(p[1..]), lc)
-    // {
-    //     foo450(p, r, k);
-    //     if |p| == 2 {
-    //         //  
-    //     } else {
-
-    //     }
-    // }
-
-    /**
-     *  Next path from a leaf must go to the next leaf
-     */
-     lemma {:induction r} nextPathNextLeaf(p: seq<bit>, r : ITree, k : nat) 
-        requires isCompleteTree(r)                              // 1.
-        requires 1 <= |p| == height(r) - 1                      // 2.
-        requires 0 <= k < |leavesIn(r)| - 1                     // 3.
-        requires nodeAt(p, r) == leavesIn(r)[k]                 // 4.
-        ensures exists i ::  0 <= i < |p| && p[i] == 0          //  P1
-        ensures  nodeAt(nextPath(p), r) == leavesIn(r)[k + 1]   //  P2
-    {
-        //  proof of P1
-        foo450(p, r, k);
-        //   proof of P2
-        nextPathIsSucc(p);
-        assert(bitListToNat(nextPath(p)) == bitListToNat(p) + 1);
-        foo200(p, r, k);
-        assert(bitListToNat(p) == k);
-        assert(bitListToNat(nextPath(p)) == k + 1);
-        foo200(nextPath(p), r, k + 1);
-
-
-    }
+   
 
 
 }
