src/dafny/smart/CompleteTrees.dfy
@@ -1,0 +1,101 @@
+/*
+ * Copyright 2020 ConsenSys AG.
+ *
+ * Licensed under the Apache License, Version 2.0 (the "License"); you may 
+ * not use this file except in compliance with the License. You may obtain 
+ * a copy of the License at http://www.apache.org/licenses/LICENSE-2.0
+ *
+ * Unless required by applicable law or agreed to in writing, software dis-
+ * tributed under the License is distributed on an "AS IS" BASIS, WITHOUT 
+ * WARRANTIES OR CONDITIONS OF ANY KIND, either express or implied. See the 
+ * License for the specific language governing permissions and limitations 
+ * under the License.
+ */
+
+include "Trees2.dfy"
+include "Helpers.dfy"
+
+/**
+ *     Provide complete trees.
+ */
+module CompleteTrees { 
+
+    import opened Trees
+    import opened Helpers
+
+    /**
+     *  Complete trees.
+     *
+     *  @param  root    The root node of the tree.
+     *  @returns        True if and only if the tree rooted at root is complete
+     */
+    predicate isCompleteTree(root : ITree) 
+        decreases root
+    {
+        match root 
+            //  A leaf is a complete tree
+            case ILeaf(_, _) => true
+            //  From a root node, a tree is complete if both children have same height
+            case INode(_, lc, rc, _) => 
+                && height(lc) == height(rc) 
+                && isCompleteTree(lc) && isCompleteTree(rc)
+    }
+
+    
+    //  Helper lemmas for complete trees.
+
+    /**
+     *  Relation between height and number of leaves in a complete tree.
+     */
+    lemma {:induction root} completeTreeNumberLemmas(root : ITree) 
+        ensures isCompleteTree(root) ==> |leavesIn(root)| == power2(height(root) - 1)
+        ensures isCompleteTree(root) ==> |nodesIn(root)| == power2(height(root)) - 1
+    {   //  Thanks Dafny
+    }
+
+    /**
+     *  Two complete tree of same height have same number of leaves.
+     */
+    lemma {:induction r1, r2} completeTreesOfSameHeightHaveSameNumberOfLeaves(r1: ITree, r2: ITree) 
+        requires isCompleteTree(r1)
+        requires isCompleteTree(r2)
+        ensures height(r1) == height(r2) ==> |leavesIn(r1)| == |leavesIn(r2)|
+    {   //  Thanks Dafny
+    }
+
+    /**
+     *  Children of a node in a complete tree have same number of leaves.
+     */
+    lemma {:induction r} completeTreesLeftRightHaveSameNumberOfLeaves(r : ITree) 
+        requires isCompleteTree(r)
+        requires height(r) >= 2
+        ensures match r
+            case INode(_, lc, rc, _) => 
+                |leavesIn(lc)| == |leavesIn(rc)| == power2(height(r) - 1) / 2
+    {
+        match r 
+            case INode(_, lc, rc, _) =>
+                completeTreesOfSameHeightHaveSameNumberOfLeaves(lc,rc);
+    }
+
+    lemma {:induction r} completeTreesLeftRightChildrenLeaves(r : ITree, h : nat) 
+        requires isCompleteTree(r)
+        requires h == height(r) >= 2
+        ensures |leavesIn(r)| == power2(h - 1)
+        ensures match r
+            case INode(_, lc, rc, _) => 
+                leavesIn(lc) == leavesIn(r)[.. power2(h - 1) / 2]
+                && leavesIn(rc) == leavesIn(r)[power2(height(r) - 1) / 2 ..]
+    {
+        if h == 2 {
+            //  Thanks Dafny
+        } else {
+            match r
+                case INode(_, lc, rc, _) => 
+                    completeTreesLeftRightHaveSameNumberOfLeaves(r);
+        }
+    }
+
+ 
+
+}
